theories/SLOT/Ensemble.v
@@ -13,11 +13,11 @@ Section defn.
   Context {S TE} `{StateSpace S TE}.
   Let T := list TE.
 
-  Class Generator (A : Type) :=
-    { unfolds_to : A -> T -> Prop;
-    }.
-
   Definition TraceEnsemble := T -> Prop.
+
+  Class Generator (A : Type) :=
+    { unfolds_to : A -> TraceEnsemble;
+    }.
 
   Definition EHoareTriple (pre : S -> Prop) (g : TraceEnsemble) (post : S -> Prop) :=
     forall t, g t ->
@@ -43,11 +43,14 @@ Section defn.
       e1 t1 -> e2 t2 ->
       Interleaving t1 t2 t ->
       Parallel e1 e2 t.
+
+  Definition EnsembleInvariant (prop : S -> Prop) (E : TraceEnsemble) : Prop :=
+    forall (t : T), E t -> TraceInvariant prop t.
 End defn.
 
 Notation "'-{{' a '}}' t '{{' b '}}'" := (EHoareTriple a t b)(at level 40) : hoare_scope.
-Infix ">>" := (TraceEnsembleConcat) (at level 100) : hoare_scope.
-Infix "|>" := (Parallel) (at level 101) : hoare_scope.
+Infix "->>" := (TraceEnsembleConcat) (at level 100) : hoare_scope.
+Infix "-||" := (Parallel) (at level 101) : hoare_scope.
 
 Section props.
   Context {S TE} `{StateSpace S TE}.
@@ -56,7 +59,7 @@ Section props.
   Lemma e_hoare_concat : forall pre mid post e1 e2,
       -{{pre}} e1 {{mid}} ->
       -{{mid}} e2 {{post}} ->
-      -{{pre}} e1 >> e2 {{post}}.
+      -{{pre}} e1 ->> e2 {{post}}.
   Proof.
     intros *. intros H1 H2 t Ht.
     destruct Ht.
@@ -64,50 +67,13 @@ Section props.
   Qed.
 
   Section perm_props.
-    Context (can_swap : TE -> TE -> Prop).
-
-    Definition perm t1 t2 := Permutation can_swap (t1 ++ t2).
-
-    Definition compatible P1 Q1 P2 Q2 t1 t2 :=
-      {{P1}} t1 {{Q1}} ->
-      {{P2}} t2 {{Q2}} ->
-      -{{P1 /\' P2}} perm t1 t2 {{Q1 /\' Q2}}.
-
-    Goal forall A B P Q R a b x,
-        compatible P Q A B [a] [x] ->
-        compatible Q R A B [b] [x] ->
-        compatible P R A B [a;b] [x].
+    Lemma e_hoare_par_seq : forall e1 e2 e P Q R,
+        -{{P}} e1 -|| e {{Q}} ->
+        -{{Q}} e2 -|| e {{R}} ->
+        -{{P}} e1 ->> e2 -|| e {{R}}.
     Proof.
-      unfold compatible, perm.
-      simpl in *.
-      intros. intros t Ht.
-Abort.
-
-    Goal forall P Q R te0 te1 te2,
-        -{{P}} perm [te0] [te1] {{Q}} ->
-        -{{Q}} perm [te0] [te2] {{R}} ->
-        -{{P}} perm [te0] [te1; te2] {{R}}.
-    Proof.
-      intros. intros t Ht.
-      destruct Ht.
-    Abort.
-
-    Lemma hoare_perm_seq : forall P Q R t0 t1 t2,
-        -{{P}} perm t0 t1 {{Q}} ->
-        -{{Q}} perm t0 t2 {{R}} ->
-        -{{P}} perm t0 (t1 ++ t2) {{R}}.
-    Abort. (* This is _likely_ wrong:
-            P t1:[a b] Q t2:[c d] R
-              t0: [A         B]
-            *)
+      intros *. intros H1 H2 t Ht s s' Hss' Hpre.
+      destruct Ht as [t1 t2 t Ht1 Ht2 Hint].
+    Abort. (* This is wrong? *)
   End perm_props.
-
-  Lemma e_hoare_par_seq : forall e1 e2 e P Q R,
-      -{{P}} e1 |> e {{Q}} ->
-      -{{Q}} e2 |> e {{R}} ->
-      -{{P}} e1 >> e2 |> e {{R}}.
-  Proof.
-    intros *. intros H1 H2 t Ht s s' Hss' Hpre.
-    destruct Ht as [t1 t2 t Ht1 Ht2 Hint].
-  Abort. (* This is wrong? *)
 End props.
