theories/SLOT/Process.v
@@ -1,11 +1,22 @@
 From Coq Require
+     List
      String
      Vector.
 
 Import String.
-Module Vec := Vector.
+Import List.
+Import List.ListNotations.
+
+From Containers Require
+     OrderedType
+     MapInterface
+     MapFacts
+     MapAVLInstance.
+
+Module Map := MapInterface.
 
 From LibTx Require Import
+     FoldIn
      SLOT.Hoare
      SLOT.Ensemble
      SLOT.EventTrace.
@@ -18,6 +29,8 @@ Section defn.
   Let PID := ctx_pid_t ctx.
   Let Req := ctx_req_t ctx.
   Let Ret := ctx_ret_t ctx.
+
+  Context `{Hord : OrderedType.OrderedType PID}.
 
   Let TE := @TraceElem ctx.
   Let T := @Trace ctx.
@@ -35,57 +48,71 @@ Section defn.
 
   Definition throw (_ : string) := t_dead.
 
-  Inductive ThreadStep (pid : PID) : Thread -> Thread -> TE -> Prop :=
-  | thread_step : forall req ret cont,
-      ThreadStep pid
-                 (t_cont req cont) (cont ret)
-                 (trace_elem _ pid req ret).
+  Definition threadStep (s s' : Thread) (te : TE) : Prop.
+    destruct te as [pid req ret].
+    destruct s as [|req' cont].
+    - exact False. (* Dead threads can't run *)
+    - refine ({Hreq : req = req' | s' = cont _}).
+      subst.
+      exact ret.
+  Defined.
 
-  Hint Constructors ThreadStep.
+  Inductive ThreadGenerator pid : Thread -> TraceEnsemble :=
+  | tg_nil : ThreadGenerator pid t_dead []
+  | tg_cons : forall req ret cont trace,
+      ThreadGenerator pid (cont ret) trace ->
+      ThreadGenerator pid (t_cont req cont) (trace_elem _ pid req ret :: trace).
 
-  Global Instance runnableThread (pid : PID) : Runnable Thread :=
-    {| runnable_step := ThreadStep pid |}.
+  Global Instance threadGen pid : Generator Thread :=
+    { unfolds_to := ThreadGenerator pid;
+    }.
+
+  Global Instance runnableThread : Runnable Thread :=
+    {| runnable_step := threadStep |}.
 
   Global Instance runnableHoare {A} `{Runnable A} : StateSpace A TE :=
-    {| chain_rule := runnable_step; |}.
+    {| chain_rule := runnable_step |}.
 
   Global Instance runnableGenerator {A} `{Runnable A} : Generator A :=
-    {| unfolds_to g t := exists g', LongStep g t g';
-    |}.
+    {| unfolds_to g t := exists g', LongStep g t g' |}.
+
+  (* Inductive ThreadsStep : Threads -> Threads -> TE -> Prop := *)
+  (* | threads_step : forall pid te threads thread' (HIn : MapInterface.In pid threads), *)
+  (*     ThreadStep pid (find' pid threads HIn) thread' te -> *)
+  (*     ThreadsStep threads (Map.add pid thread' threads) te. *)
 End defn.
 
-Section ComposeSystems.
-  Context {ctx : Ctx} {sys1 sys2 : Type} `{@Runnable ctx sys1} `{@Runnable ctx sys2}.
+(* Section ComposeSystems. *)
+(*   Context {ctx : Ctx} {sys1 sys2 : Type} `{@Runnable ctx sys1} `{@Runnable ctx sys2}. *)
 
-  Let S : Type := sys1 * sys2.
+(*   Let S : Type := sys1 * sys2. *)
 
-  Inductive composeRunnableStep : S -> S -> _ -> Prop :=
-  | cr_step_l : forall s_l s_l' s_r te,
-      runnable_step s_l s_l' te ->
-      composeRunnableStep (s_l, s_r) (s_l', s_r) te
-  | cr_step_r : forall s_r s_r' s_l te,
-      runnable_step s_r s_r' te ->
-      composeRunnableStep (s_l, s_r) (s_l, s_r') te.
+(*   Inductive composeRunnableStep : S -> S -> _ -> Prop := *)
+(*   | cr_step_l : forall s_l s_l' s_r te, *)
+(*       runnable_step s_l s_l' te -> *)
+(*       composeRunnableStep (s_l, s_r) (s_l', s_r) te *)
+(*   | cr_step_r : forall s_r s_r' s_l te, *)
+(*       runnable_step s_r s_r' te -> *)
+(*       composeRunnableStep (s_l, s_r) (s_l, s_r') te. *)
 
-  Global Instance composeRunnable  :
-    @Runnable ctx (sys1 * sys2) :=
-    {| runnable_step := composeRunnableStep |}.
-End ComposeSystems.
+(*   Global Instance composeRunnable  : *)
+(*     @Runnable ctx (sys1 * sys2) := *)
+(*     {| runnable_step := composeRunnableStep |}. *)
+(* End ComposeSystems. *)
 
-Section ReplicateSystem.
-  Context {ctx : Ctx} {sys : Type} `{Runnable ctx sys}.
+(* Section ReplicateSystem. *)
+(*   Context {ctx : Ctx} {sys : Type} `{Runnable ctx sys}. *)
 
-  Definition replicated {t} (N : nat) create : Vec.t t N :=
-    Vec.map create (FoldIn.seq_vec N).
+(*   Definition replicated {t} (N : nat) create : Vec.t t N := *)
+(*     Vec.map create (FoldIn.seq_vec N). *)
 
-  Inductive replRunnableStep {N : nat} : Vec.t sys N -> Vec.t sys N -> _ -> Prop :=
-  | repl_run_step : forall i vec s s' te,
-      Vec.nth vec i = s ->
-      runnable_step s s' te ->
-      replRunnableStep vec (Vec.replace vec i s') te.
+(*   Inductive replRunnableStep {N : nat} : Vec.t sys N -> Vec.t sys N -> _ -> Prop := *)
+(*   | repl_run_step : forall i vec s s' te, *)
+(*       Vec.nth vec i = s -> *)
+(*       runnable_step s s' te -> *)
+(*       replRunnableStep vec (Vec.replace vec i s') te. *)
 
-  Global Instance replicatedRunnable `{@Runnable ctx sys} {N} :
-    @Runnable ctx (Vec.t sys N) :=
-    {| runnable_step := replRunnableStep;
-    |}.
-End ReplicateSystem.
+(*   Global Instance replicatedRunnable `{@Runnable ctx sys} {N} : *)
+(*     @Runnable ctx (Vec.t sys N) := *)
+(*     {| runnable_step := replRunnableStep; |}. *)
+(* End ReplicateSystem. *)
